much more efficient and cleaner dio auto tactic the only problem is that the size of generate formula is increase at each cleaning changing atoms to elem simplified lost of proofs but got me much bigger encodings in the end ... it does really matter since efficiency is not the objective here

theories/H10/Dio/dio_bounded.v
@@ -90,7 +90,7 @@ Section df_mconj.
     destruct H as (f & Hf).
     exists (df_mconj k f).
     abstract(intros v; rewrite df_mconj_spec; split;
-      intros E i Hi; generalize (E _ Hi); apply Hf; trivial). 
+      intros E i Hi; generalize (E _ Hi); apply Hf; trivial).
   Defined.
 
 End df_mconj.
@@ -123,20 +123,20 @@ Section dio_bounded_fall.
 
     Local Fact dio_rel_dc_Code c : 𝔻R (dc_Code c).
     Proof. 
-      destruct c as (u & [ n | v | [] | [] v w ]); unfold dc_Code; dio_rel_auto.
+      destruct c as (u & [ n | v | [] | [] v w ]); unfold dc_Code; dio auto.
     Defined.
 
     Hint Resolve dio_rel_dc_Code : dio_rel_db.
 
-    (* 
+    (*
 
       Eval compute in df_size_Z (proj1_sig (dio_rel_dc_Code (0,dee_comp do_mul 1 2))). 
 
     *)
 
-    (* Case of do_mul gives the overall bound of 778551 
+    (* Case of do_mul gives the overall bound of 962535 
 
-    Let dc_Code_size_Z c : (df_size_Z (proj1_sig (dio_rel_dc_Code c)) <= 778551)%Z.
+    Let dc_Code_size_Z c : (df_size_Z (proj1_sig (dio_rel_dc_Code c)) <= 962535)%Z.
     Proof.
       destruct c as (u & [ n | v | [] | [] v w ]); compute; discriminate.
     Qed. *)
@@ -149,12 +149,13 @@ Section dio_bounded_fall.
         i > k+2   |          |       |  i-(k+2)  *)
 
     Local Fact dc_Code_spec c φ π ν ω : 
-                                 (forall i, i < k -> is_cipher_of (ν 0) (π iq) (φ i) (π i))
-                              -> (is_cipher_of (ν 0) (π iq) (fun n => n) (π k))
-                              -> (forall x, dc_vars c x -> x < k)
-                              -> (forall i, i < il -> ω i = π i)
-                              -> (forall i, il <= i -> ω i = ν (i-il))
-                             -> dc_Code c ω <-> forall j, j < ν 0 -> dc_eval (fun i => φ i j) (dv_lift ν j) c.
+          (forall i, i < k -> is_cipher_of (ν 0) (π iq) (φ i) (π i))
+       -> (is_cipher_of (ν 0) (π iq) (fun n => n) (π k))
+       -> (forall x, dc_vars c x -> x < k)
+       -> (forall i, i < il -> ω i = π i)
+       -> (forall i, il <= i -> ω i = ν (i-il))
+       -> dc_Code c ω 
+      <-> forall j, j < ν 0 -> dc_eval (fun i => φ i j) (dv_lift ν j) c.
     Proof.
       intros G1 G2 G3 G4 G5.
       assert (ω il = ν 0) as G0.
@@ -210,18 +211,18 @@ Section dio_bounded_fall.
     Local Definition dc_list_Code ll ν := fold_right (fun c P => dc_Code c ν /\ P) True ll.
 
     Local Fact dio_rel_dc_list_Code ll : 𝔻R (dc_list_Code ll).
-    Proof. induction ll; unfold dc_list_Code; simpl; dio_rel_auto. Qed.
+    Proof. induction ll; unfold dc_list_Code; simpl; dio auto. Qed.
 
     Hint Resolve dio_rel_dc_list_Code : dio_rel_db.
 
     Local Fact dc_list_Code_spec ll φ π ν ω : 
-                                       (forall i, i < k -> is_cipher_of (ν 0) (π iq) (φ i) (π i))
-                                    -> (is_cipher_of (ν 0) (π iq) (fun n => n) (π k))
-                                    -> (forall c, In c ll -> forall x, dc_vars c x -> x < k)
-                                    -> (forall i, i < il  -> ω i = π i)
-                                    -> (forall i, il <= i -> ω i = ν (i-il))
-                                    -> dc_list_Code ll ω 
-                                   <-> forall j, j < ν 0 -> Forall (dc_eval (fun i => φ i j) (dv_lift ν j)) ll.
+          (forall i, i < k -> is_cipher_of (ν 0) (π iq) (φ i) (π i))
+       -> (is_cipher_of (ν 0) (π iq) (fun n => n) (π k))
+       -> (forall c, In c ll -> forall x, dc_vars c x -> x < k)
+       -> (forall i, i < il  -> ω i = π i)
+       -> (forall i, il <= i -> ω i = ν (i-il))
+       -> dc_list_Code ll ω 
+      <-> forall j, j < ν 0 -> Forall (dc_eval (fun i => φ i j) (dv_lift ν j)) ll.
     Proof.
       intros G1 G2 G3 G4 G5; revert G3.
       rewrite <- Forall_forall.
@@ -234,12 +235,14 @@ Section dio_bounded_fall.
             rewrite Forall_cons_inv in E1; tauto.
     Qed.
 
-    Local Definition ciphers ν := CodeNat (ν il) (ν iq) (ν k) /\ forall i, i < k -> Code (ν il) (ν iq) (ν i).
+    Local Definition ciphers ν := 
+             CodeNat (ν il) (ν iq) (ν k) 
+          /\ forall i, i < k -> Code (ν il) (ν iq) (ν i).
 
     Local Fact dio_rel_ciphers : 𝔻R ciphers.
     Proof.
-      unfold ciphers; dio_rel_auto. 
-      apply dio_rel_mconj; intros; dio_rel_auto.
+      unfold ciphers; dio auto.
+      apply dio_rel_mconj; intros; dio auto.
     Defined.
 
     Hint Resolve dio_rel_ciphers : dio_rel_db.
@@ -264,14 +267,15 @@ Section dio_bounded_fall.
     Let pre_quant ν := ν il+1 < ν iq /\ ciphers ν /\ dc_list_Code ll ν.
 
     Let dio_rel_pre_quant : dio_rel pre_quant.
-    Proof. unfold pre_quant; dio_rel_auto. Defined.
+    Proof. unfold pre_quant; dio auto. Defined.
 
     Definition dc_list_bfall ν := exists π, pre_quant (fun i => if le_lt_dec il i then ν (i-il) else π i).
 
     Let dc_list_bfall_spec_1 ν :
-          dc_list_bfall ν <-> exists q φ, ν 0+1 < q 
-                                      /\ (forall i j, i < k -> j < ν 0 -> φ i j < power q 2) 
-                                      /\ forall j, j < ν 0 -> Forall (dc_eval (fun i => φ i j) (dv_lift ν j)) ll.
+            dc_list_bfall ν 
+        <-> exists q φ, ν 0+1 < q 
+                    /\ (forall i j, i < k -> j < ν 0 -> φ i j < power q 2) 
+                    /\  forall j, j < ν 0 -> Forall (dc_eval (fun i => φ i j) (dv_lift ν j)) ll.
     Proof.
       split.
       + intros (pi & G0 & G1 & G4).
@@ -321,7 +325,9 @@ Section dio_bounded_fall.
             intros i Hi; destruct (le_lt_dec il i); auto; omega.
     Qed.
 
-    Let dc_list_bfall_spec ν : (forall i, i < ν 0 -> exists φ, Forall (dc_eval φ (dv_lift ν i)) ll) <-> dc_list_bfall ν .
+    Let dc_list_bfall_spec ν : 
+            (forall i, i < ν 0 -> exists φ, Forall (dc_eval φ (dv_lift ν i)) ll) 
+        <-> dc_list_bfall ν .
     Proof.
       rewrite dc_list_bfall_spec_1; split.
       + intros H.
@@ -353,20 +359,20 @@ Section dio_bounded_fall.
       unfold dc_list_bfall.
       destruct dio_rel_pre_quant as (f & Hf).
       eexists (df_mexists il f).
-      intros; rewrite df_mexists_spec; split;
-      intros (phi & H); exists phi; revert H; rewrite <- Hf; auto.
+      abstract(intros; rewrite df_mexists_spec; split;
+        intros (phi & H); exists phi; revert H; rewrite <- Hf; auto).
     Defined.
 
   End dio_bounded_elem.
 
-  Theorem dio_bounded_fall P : dio_rel P -> dio_rel (fun ν => forall i, i < ν 0 -> P (dv_lift ν i)).
+  Theorem dio_bounded_fall P : 𝔻R P -> 𝔻R (fun ν => forall i, i < ν 0 -> P (dv_lift ν i)).
   Proof.
     intros (f & Hf).
     destruct (dio_formula_elem f) as (ll & H1 & H2 & H3).
     revert H2; generalize (4*df_size f); intros k H2.
     generalize (dio_rel_dc_list_bfall _ H2).
     apply dio_rel_equiv; intros v.
-    split; intros H i Hi; generalize (H _ Hi); rewrite <- Hf, H3; auto.
+    abstract(split; intros H i Hi; generalize (H _ Hi); rewrite <- Hf, H3; auto).
   Defined.
 
 End dio_bounded_fall.
@@ -385,18 +391,17 @@ Section dfbfall.
 
   Let rho i := match i with 0 => 0 | S i => S (S i) end. 
 
-  Let dfbfall_full : dio_rel (fun ν => forall i, i < ν 0 -> df_pred f (dv_change ν i)).
+  Let dfbfall_full : 𝔻R (fun ν => forall i, i < ν 0 -> df_pred f (dv_change ν i)).
   Proof.
     assert (dio_rel (df_pred (df_ren rho f))) as H.
     { exists (df_ren rho f); tauto. }
     destruct (dio_bounded_fall H) as (g & Hg).
     exists g.
-    intros v.
-    rewrite Hg. 
-    split; intros G i Hi; generalize (G _ Hi);  
-      rewrite df_pred_ren; apply df_pred_ext;
-      intros [ | [ | x ] ]; simpl; auto.
-  Qed.
+    abstract (intros v; rewrite Hg; 
+      split; intros G i Hi; generalize (G _ Hi);
+        rewrite df_pred_ren; apply df_pred_ext;
+        intros [ | [ | x ] ]; simpl; auto).
+  Defined.
 
   Definition dfbfall := proj1_sig dfbfall_full.
 
@@ -435,7 +440,7 @@ Corollary dio_rel_fall_lt_bound a (K : nat -> nat -> (nat -> nat) -> Prop) :
            𝔻P a
    -> 𝔻R (fun ν => K (ν 0) (a ν↓) ν↓) 
    -> 𝔻R (fun ν => forall x, x < a ν -> K x (a ν) ν).
-Proof. intros; dio_rel_auto. Defined.
+Proof. intros; dio auto. Defined.
 
 Hint Resolve dio_rel_fall_lt_bound : dio_rel_db.
 
